cleaned graph lib

Network_Security_Policy_Verification/Lib/FiniteGraph.thy
@@ -6,8 +6,8 @@ begin
 
 section {*Specification of a finite directed graph*}
 
-text{* A graph G=(V,E) consits of a set of vertices V, also called nodes, 
-       and a set of edges E. The edges are tuples of vertices. Both, 
+text{* A graph @{text "G=(V,E)"} consits of a set of vertices @{text V}, also called nodes, 
+       and a set of edges @{text E}. The edges are tuples of vertices. Both, 
        the set of vertices and edges is finite. *}
 
 (* Inspired by
@@ -16,7 +16,8 @@ Author: Benedikt Nordhoff and Peter Lammich
 http://afp.sourceforge.net/entries/Dijkstra_Shortest_Path.shtml
 *)
 
-section {* Definitions *}
+section {* Graph  *}
+subsection{*Definitions*}
   text {* A graph is represented by a record. *}
   record 'v graph =
     nodes :: "'v set"
@@ -25,7 +26,7 @@ section {* Definitions *}
   text {* In a well-formed graph, edges only go from nodes to nodes. *}
   locale wf_graph = 
     fixes G :: "'v graph"
-    -- "Edges only refernce to existing nodes"
+    -- "Edges only reference to existing nodes"
     assumes E_wf: "fst ` (edges G) \<subseteq> (nodes G)"
                      "snd ` (edges G) \<subseteq> (nodes G)"
     and finiteE: "finite (edges G)" (*implied by finiteV*)
@@ -48,10 +49,8 @@ section {* Definitions *}
   end
 
 subsection {* Basic operations on Graphs *}
-
- 
   text {* The empty graph. *}
-  definition empty where 
+  definition empty :: "'v graph" where 
     "empty \<equiv> \<lparr> nodes = {}, edges = {} \<rparr>"
 
   text {* Adds a node to a graph. *}
@@ -60,38 +59,40 @@ subsection {* Basic operations on Graphs *}
 
   text {* Deletes a node from a graph. Also deletes all adjacent edges. *}
   definition delete_node where "delete_node v G \<equiv> \<lparr> 
-    nodes = (nodes G) - {v},   
-    edges = {(e1, e2). (e1, e2) \<in> edges G \<and> e1 \<noteq> v \<and> e2 \<noteq> v}
+      nodes = (nodes G) - {v},   
+      edges = {(e1, e2). (e1, e2) \<in> edges G \<and> e1 \<noteq> v \<and> e2 \<noteq> v}
     \<rparr>"
 
   text {* Adds an edge to a graph. *}
   definition add_edge where 
   "add_edge v v' G = \<lparr>nodes = nodes G \<union> {v,v'}, edges = {(v, v')} \<union> edges G \<rparr>"
 
-
   text {* Deletes an edge from a graph. *}
-  definition delete_edge where "delete_edge v v' G \<equiv> \<lparr>nodes = nodes G, 
-    edges = {(e1,e2). (e1, e2) \<in> edges G \<and> (e1,e2) \<noteq> (v,v')} \<rparr>"
+  definition delete_edge where "delete_edge v v' G \<equiv> \<lparr>
+      nodes = nodes G, 
+      edges = {(e1,e2). (e1, e2) \<in> edges G \<and> (e1,e2) \<noteq> (v,v')}
+    \<rparr>"
   
   definition delete_edges::"'v graph \<Rightarrow> ('v \<times> 'v) set \<Rightarrow> 'v graph" where 
-    "delete_edges G es = \<lparr>nodes = nodes G, 
-    edges = {(e1,e2). (e1, e2) \<in> edges G \<and> (e1,e2) \<notin> es} \<rparr>"
+    "delete_edges G es \<equiv> \<lparr>
+      nodes = nodes G, 
+      edges = {(e1,e2). (e1, e2) \<in> edges G \<and> (e1,e2) \<notin> es}
+    \<rparr>"
 
   fun delete_edges_list::"'v graph \<Rightarrow> ('v \<times> 'v) list \<Rightarrow> 'v graph" where 
     "delete_edges_list G [] = G"|
     "delete_edges_list G ((v,v')#es) = delete_edges_list (delete_edge v v' G) es"
 
-
   definition fully_connected :: "'v graph \<Rightarrow> 'v graph" where
     "fully_connected G \<equiv> \<lparr>nodes = nodes G, edges = nodes G \<times> nodes G \<rparr>"
 
 
-text {* extended graph operations *}
-  text {* Reflexive transitive successors of a node. Or: All reachable nodes for v including v. *}
+text {* Extended graph operations *}
+  text {* Reflexive transitive successors of a node. Or: All reachable nodes for @{text v} including @{text v}. *}
   definition succ_rtran :: "'v graph \<Rightarrow> 'v \<Rightarrow> 'v set" where
     "succ_rtran G v = {e2. (v,e2) \<in> (edges G)\<^sup>*}"
 
-  text {* Transitive successors of a node. Or: All reachable nodes for v. *}
+  text {* Transitive successors of a node. Or: All reachable nodes for @{text v}. *}
   definition succ_tran :: "'v graph \<Rightarrow> 'v \<Rightarrow> 'v set" where
     "succ_tran G v = {e2. (v,e2) \<in> (edges G)\<^sup>+}"
 
@@ -110,25 +111,23 @@ text {* extended graph operations *}
     thus "finite (succ_tran G v)" using succ_tran_def by metis
   qed
   
-  text{* If there is no edge leaving from v, then v has no successors *}
+  text{* If there is no edge leaving from @{text v}, then @{text v} has no successors *}
   lemma succ_tran_empty: "\<lbrakk> wf_graph G; v \<notin> (fst ` edges G) \<rbrakk> \<Longrightarrow> succ_tran G v = {}"
-  by (metis (lifting) Collect_empty_eq Domain.DomainI converse_tranclE fst_eq_Domain succ_tran_def)
+    unfolding succ_tran_def using image_iff tranclD by fastforce
 
-  text{* succ_tran is subset of nodes *}
+  text{* @{const succ_tran} is subset of nodes *}
   lemma succ_tran_subseteq_nodes: "\<lbrakk> wf_graph G \<rbrakk> \<Longrightarrow> succ_tran G v \<subseteq> nodes G"
-    apply(simp add: succ_tran_def)
-    by (metis (lifting) mem_Collect_eq subsetI trancl.cases wf_graph.E_wfD(2))
+    unfolding succ_tran_def using tranclD2 wf_graph.E_wfD(2) by fastforce
 
-
-  text {* The number of reachable nodes from v *}
+  text {* The number of reachable nodes from @{text v} *}
   definition num_reachable :: "'v graph \<Rightarrow> 'v \<Rightarrow> nat" where
     "num_reachable G v = card (succ_tran G v)"
 
   definition num_reachable_norefl :: "'v graph \<Rightarrow> 'v \<Rightarrow> nat" where
     "num_reachable_norefl G v = card (succ_tran G v - {v})"
 
-  text{*card returns 0 for infinite sets. Here, for a well-formed graph, if num_reachable is zero,
-        there are actually no nodes reachable.*}
+  text{*@{const card} returns @{term 0} for infinite sets.
+        Here, for a well-formed graph, if @{const num_reachable} is zero, there are actually no nodes reachable.*}
   lemma num_reachable_zero: "\<lbrakk>wf_graph G; num_reachable G v = 0\<rbrakk> \<Longrightarrow> succ_tran G v = {}"
   apply(unfold num_reachable_def)
   apply(case_tac "finite (succ_tran G v)")
@@ -136,8 +135,8 @@ text {* extended graph operations *}
   apply(blast intro: succ_tran_finite)
   done
   lemma num_succtran_zero: "\<lbrakk>succ_tran G v = {}\<rbrakk> \<Longrightarrow> num_reachable G v = 0"
-  by(unfold num_reachable_def, simp)
-  lemma num_reachable_zero_iff: "\<lbrakk>wf_graph G\<rbrakk> \<Longrightarrow> (num_reachable G v = 0) <-> (succ_tran G v = {})"
+    unfolding num_reachable_def by simp
+  lemma num_reachable_zero_iff: "\<lbrakk>wf_graph G\<rbrakk> \<Longrightarrow> (num_reachable G v = 0) \<longleftrightarrow> (succ_tran G v = {})"
   by(metis num_succtran_zero num_reachable_zero)
 
 
@@ -152,10 +151,9 @@ subsection{*undirected graph simulation*}
   definition undirected :: "'v graph \<Rightarrow> 'v graph"
     where "undirected G = \<lparr> nodes = nodes G, edges = (edges G) \<union> {(b,a). (a,b) \<in> edges G} \<rparr>"
 
-section {*Lemmata*}
+section {*Graph Lemmas*}
 
-  lemma graph_eq_intro: "(nodes (G::'a graph) = nodes G') \<Longrightarrow> (edges G = edges G') \<Longrightarrow> G = G'"
-  by simp
+  lemma graph_eq_intro: "(nodes (G::'a graph) = nodes G') \<Longrightarrow> (edges G = edges G') \<Longrightarrow> G = G'" by simp
 
   -- "finite"
   lemma wf_graph_finite_filterE: "wf_graph G \<Longrightarrow> finite {(e1, e2). (e1, e2) \<in> edges G \<and> P e1 e2}"
@@ -170,34 +168,31 @@ section {*Lemmata*}
   lemma edges_empty[simp]: "edges empty = {}" unfolding empty_def by simp
 
   -- "add node"
-  lemma add_node_wf[simp]:
-    "wf_graph g \<Longrightarrow> wf_graph (add_node v g)"
-      unfolding add_node_def
-      unfolding wf_graph_def
-      by (auto)
+  lemma add_node_wf[simp]: "wf_graph g \<Longrightarrow> wf_graph (add_node v g)"
+    unfolding add_node_def wf_graph_def by (auto)
 
-  lemma delete_node_wf[simp]:
-  "wf_graph G \<Longrightarrow> wf_graph (delete_node v G)"
-  by(auto simp add: delete_node_def wf_graph_def wf_graph_finite_filterE)
+  lemma delete_node_wf[simp]: "wf_graph G \<Longrightarrow> wf_graph (delete_node v G)"
+    by(auto simp add: delete_node_def wf_graph_def wf_graph_finite_filterE)
 
   -- "add edgde"
   lemma add_edge_wf[simp]: "wf_graph G \<Longrightarrow> wf_graph (add_edge v v' G)"
-  by(auto simp add: add_edge_def add_node_def wf_graph_def)
+    by(auto simp add: add_edge_def add_node_def wf_graph_def)
 
   -- "delete edge"
   lemma delete_edge_wf[simp]: "wf_graph G \<Longrightarrow> wf_graph (delete_edge v v' G)"
-  by(auto simp add: delete_edge_def add_node_def wf_graph_def split_def)
+    by(auto simp add: delete_edge_def add_node_def wf_graph_def split_def)
  
   -- "delte edges"
   lemma delete_edges_list_wf[simp]: "wf_graph G \<Longrightarrow> wf_graph (delete_edges_list G E)"
     by(induction E arbitrary: G, simp, force)
   lemma delete_edges_wf[simp]: "wf_graph G \<Longrightarrow> wf_graph (delete_edges G E)"
-  by(auto simp add: delete_edges_def add_node_def wf_graph_def split_def)
+    by(auto simp add: delete_edges_def add_node_def wf_graph_def split_def)
   lemma delete_edges_list_set: "delete_edges_list G E = delete_edges G (set E)"
-    apply(induction E arbitrary: G)
-     apply(simp_all add: delete_edges_def)
-    apply(clarify)
-    by(simp add: delete_edge_def)
+    proof(induction E arbitrary: G)
+    case Nil thus ?case by (simp add: delete_edges_def)
+    next
+    case (Cons e E) thus ?case by(cases e)(simp add: delete_edge_def delete_edges_def)
+    qed
   lemma delete_edges_list_union: "delete_edges_list G (ff @ keeps) = delete_edges G (set ff \<union> set keeps)"
    by(simp add: delete_edges_list_set)
   lemma add_edge_delete_edges_list: 
@@ -215,19 +210,15 @@ section {*Lemmata*}
     by(simp add: delete_edges_simp2)
 
  --"add delete"
-  lemma add_delete_edge: "wf_graph (G::'a graph) \<Longrightarrow> (a,b) \<in> edges G \<Longrightarrow> 
-  add_edge a b (delete_edge a b G) = G"
+  lemma add_delete_edge: "wf_graph (G::'a graph) \<Longrightarrow> (a,b) \<in> edges G \<Longrightarrow> add_edge a b (delete_edge a b G) = G"
    apply(simp add: delete_edge_def add_edge_def wf_graph_def)
-   apply(clarify)
-   apply(rule graph_eq_intro)
-    by (auto)
+   apply(intro graph_eq_intro)
+    by auto
 
   lemma add_delete_edges: "wf_graph (G::'v graph) \<Longrightarrow> (a,b) \<in> edges G \<Longrightarrow> (a,b) \<notin> fs \<Longrightarrow>
-  add_edge a b (delete_edges G (insert (a, b) fs)) = (delete_edges G fs)"
-  apply(simp add: delete_edges_simp2 add_edge_def wf_graph_def)
-  apply(clarify)
-  apply(auto)
-  done
+    add_edge a b (delete_edges G (insert (a, b) fs)) = (delete_edges G fs)"
+    by(auto simp add: delete_edges_simp2 add_edge_def wf_graph_def)
+
 
  --"fully_connected"
   lemma fully_connected_simp: "fully_connected \<lparr>nodes = N, edges = ignore \<rparr>\<equiv> \<lparr>nodes = N, edges = N \<times> N \<rparr>"
@@ -276,7 +267,7 @@ section {*Lemmata*}
     using [[simproc add: finite_Collect]] by(simp add: backflows_def) 
   lemma backflows_minus_backflows: "backflows (X - backflows Y) = (backflows X) - Y"
     by(auto simp add: backflows_def)
-  lemma backflows_subseteq: "X \<subseteq> Y <-> backflows X \<subseteq> backflows Y"
+  lemma backflows_subseteq: "X \<subseteq> Y \<longleftrightarrow> backflows X \<subseteq> backflows Y"
     by(auto simp add: backflows_def)
   lemma backflows_un: "backflows (A \<union> B) = (backflows A) \<union> (backflows B)"
     by(auto simp add: backflows_def)
@@ -284,10 +275,6 @@ section {*Lemmata*}
     by(auto simp add: backflows_def)
   lemma backflows_alt_fstsnd: "backflows E = (\<lambda>e. (snd e, fst e)) ` E"
     by(auto simp add: backflows_def, force)
-
-
-
-
 
 
 lemmas graph_ops=add_node_def delete_node_def add_edge_def delete_edge_def delete_edges_simp2
@@ -308,9 +295,6 @@ lemmas graph_ops=add_node_def delete_node_def add_edge_def delete_edge_def delet
   lemma wf_graph_add_subset_edges: "\<lbrakk> wf_graph \<lparr> nodes = V, edges = E \<rparr>; E' \<subseteq> E \<rbrakk> \<Longrightarrow>
      wf_graph \<lparr> nodes = V, edges= E \<union> E'\<rparr>"
     by(auto simp add: wf_graph_def) (metis rev_finite_subset)
-
-
-
 
 
 (*Inspired by 
